verif/trie/common.v
@@ -1,6 +1,22 @@
 (** * common.v : Common definitions *)
 Require Import VST.floyd.functional_base.
 
+Module Type KEY_TYPE.
+  Parameter type: Type.
+End KEY_TYPE.
+
+Module Type ORD_KEY_TYPE <: KEY_TYPE.
+  Include KEY_TYPE.
+  Parameter lt: type -> type -> Prop.
+  Notation "A < B" := (lt A B).
+  Notation "A >= B" := (~ (lt A B)).
+  Parameter lt_dec: forall (x y: type), {x < y} + {x >= y}.
+  Axiom lt_trans: forall (x y z: type), x < y -> y < z -> x < z.
+  Axiom lt_neq: forall (x y: type), x < y -> x <> y.
+  Axiom ge_neq_lt: forall (x y: type), y >= x -> x <> y -> x < y.
+  Parameter EqDec: EqDec type.
+End ORD_KEY_TYPE.
+
 Definition string := list byte.
 Instance EqDec_string: EqDec string := list_eq_dec Byte.eq_dec.
 
